src/Computation/IfDec.v
@@ -1,0 +1,83 @@
+Require Import
+        Fiat.Common
+        Fiat.Computation.Decidable
+        Fiat.Computation.Core
+        Fiat.Computation.Refinements.General
+        Fiat.Computation.Monad
+        Fiat.Computation.Refinements.General.
+
+Local Open Scope comp.
+Definition IfDec_Then_Else {A} (P : Prop) (t e : Comp A) :=
+  b <- { b | decides b P}; if b then t else e.
+Arguments IfDec_Then_Else {A} P t e _ : simpl never.
+
+Notation "'IfDec' P 'Then' t 'Else' e" :=
+  (IfDec_Then_Else P t e) (at level 70) : comp_scope.
+
+Lemma refine_IfDec
+  : forall (P : Prop) b ResultT (t e : Comp ResultT),
+    decides b P
+    -> refine (IfDec P Then t Else e) (If b Then t Else e).
+Proof.
+  intros.
+  unfold IfDec_Then_Else.
+  refine pick val b; eauto.
+  rewrite refineEquiv_bind_unit; reflexivity.
+Qed.
+
+Corollary refine_IfDec_true
+  : forall (P : Prop) ResultT (t e : Comp ResultT),
+  P -> refine (IfDec P Then t Else e) t.
+Proof.
+  intros; rewrite refine_IfDec with (b := true); simpl; eauto.
+  reflexivity.
+Qed.
+
+Corollary refine_IfDec_false
+  : forall (P : Prop) ResultT (t e : Comp ResultT),
+    ~ P -> refine (IfDec P Then t Else e) e.
+Proof.
+  intros; rewrite refine_IfDec with (b := false); simpl; eauto.
+  reflexivity.
+Qed.
+
+Lemma refine_IfDec_decides :
+  forall `{Decidable P} ResultT (t e : Comp ResultT),
+    refineEquiv (IfDec P Then t Else e)
+                (If Decidable_witness Then t Else e).
+Proof.
+  split; intros.
+  - apply refine_IfDec; eauto.
+    case_eq (@Decidable_witness _ H); simpl.
+    + intros; eapply Decidable_spec; eauto.
+    + intros; eapply Decidable_complete_alt; eauto.
+  - unfold IfDec_Then_Else, If_Then_Else, refine;
+      intros; computes_to_inv.
+    destruct v0.
+    + simpl in H0; apply Decidable_spec in H0; rewrite H0; eauto.
+    + simpl in H0; eapply Decidable_sound_alt in H0; rewrite H0; eauto.
+Qed.
+
+Add Parametric Morphism A P
+  : (IfDec_Then_Else P)
+    with signature (@refine A)
+                     ==> (@refine A)
+                     ==> (@refine A)
+  as refine_IfDec_Then_Else.
+Proof.
+  intros.
+  unfold IfDec_Then_Else; f_equiv; intro.
+  rewrite !refine_if_If.
+  rewrite H0, H.
+  apply refine_PreOrder.
+Qed.
+
+(*Lemma refine_IfDec_Then_Else_ret :
+  forall P ResultT (t e : ResultT),
+    refine (IfDec P Then ret t Else ret e)
+           (ret (IfDec P Then t Else e)%comp).
+Proof.
+  intros.
+  unfold IfDec_Then_Else.
+  setoid_rewrite refine_If_Then_Else_ret; trivial.
+Qed. *)
